Redefining the CG.

src/Phasers/PhaseOrdering/CG.v
@@ -3,6 +3,7 @@ Require Import Coq.Lists.List.
 Require Import Aniceto.Pair.
 Require Import Aniceto.List.
 
+Require Import Regmode.
 Require Import Vars.
 Require Import Node.
 
@@ -10,63 +11,430 @@ Section Defs.
 
   Inductive op :=
   | ASYNC : tid -> op
-  | ASYNC_PHASED : tid -> op
-  | SIGNAL: nat -> op
-  | WAIT: nat -> op
-  | DROP: nat -> op
-  | PREC : op
+  | ASYNC_PHASED : tid -> regmode -> op
+  | SIGNAL: op
+  | WAIT: op
+  | DROP: op
   | CONTINUE: op.
 
   Definition event := (tid * op) % type.
 
   Notation edge := (node * node) %type.
 
-  Inductive Phase ph : op -> Prop :=
-  | phase_signal:
-    Phase ph (SIGNAL ph)
-  | phase_drop:
-    Phase ph (DROP ph).
+  Inductive IsSeq : op -> Prop :=
+  | is_seq_signal: IsSeq SIGNAL
+  | is_seq_wait: IsSeq WAIT
+  | is_seq_drop: IsSeq DROP
+  | is_seq_continue: IsSeq CONTINUE.
 
-  Inductive Sync ph : (op * edge) -> node -> Prop:=
-  | sync_def:
-    forall o n n',
-    Phase ph o ->
-    Sync ph (o, (n, n')) n.
+  Inductive IsPar : op -> tid -> Prop :=
+  | is_par_async: forall x, IsPar (ASYNC x) x
+  | is_par_phased: forall x r, IsPar (ASYNC_PHASED x r) x.
 
-  Inductive WaitEdge (vs:list tid) ph (es:list (op * edge)) : op * edge -> Prop :=
-  | wait_edge_def:
-    forall e n',
-    In e es ->
-    Sync ph e n' ->
-    WaitEdge vs ph es (PREC, (n',fresh vs)).
+  Let is_par o :=
+  match o with
+  | ASYNC x => Some x
+  | ASYNC_PHASED x _ => Some x
+  | _ => None
+  end.
 
-  Inductive Add vs (es:list (op*edge)) : event ->  list tid -> list (op * edge) -> Prop :=
-  | add_async:
-    forall x y n vs' es',
-    Add vs es (x, CONTINUE) vs' es' ->
-    MapsTo x n vs -> 
-    Add vs es (x, ASYNC y) (y::vs') ((ASYNC y, (n, fresh vs')) :: es')
-  | add_async_phased:
-    forall x y vs' es' e,
-    Add vs es (x, ASYNC y) vs' ((ASYNC y, e)::es') ->
-    Add vs es (x, ASYNC_PHASED y) vs' ((ASYNC_PHASED y, e)::es')
-  | add_signal:
-    forall x vs' ph e,
-    Add vs es (x, CONTINUE) vs' ((CONTINUE,e)::es) ->
-    Add vs es (x, SIGNAL ph) vs' ((SIGNAL ph, e)::es)
-  | add_wait:
-    forall x ph vs' es' e,
-    Add vs es (x, CONTINUE) vs' ((CONTINUE,e)::es) ->
-    Forall (fun e => WaitEdge vs ph es e) es' ->
-    Add vs es (x, WAIT ph) vs' (es' ++ (WAIT ph,e):: es)
-  | add_drop:
-    forall x vs' e n,
-    Add vs es (x, CONTINUE) vs' ((CONTINUE, e)::es) ->
-    Add vs es (x, DROP n) vs' ((DROP n,e):: es)
-  | add_continue:
-    forall x n,
+  Let is_par_some:
+    forall o x,
+    is_par o = Some x ->
+    IsPar o x.
+  Proof.
+    intros.
+    destruct o; simpl in *; inversion H; subst; auto using is_par_async, is_par_phased.
+  Qed.
+
+  Let is_pair_some_prop:
+    forall o x,
+    IsPar o x ->
+    is_par o = Some x.
+  Proof.
+    intros.
+    inversion H; auto.
+  Qed.
+
+  Let is_pair_some_spec:
+    forall o x,
+    is_par o = Some x <-> IsPar o x.
+  Proof.
+    split; auto.
+  Qed.
+
+  Let is_par_none:
+    forall o,
+    is_par o = None ->
+    IsSeq o.
+  Proof.
+    intros.
+    destruct o; simpl in *; inversion H; subst;
+    auto using is_seq_signal, is_seq_drop, is_seq_continue, is_seq_wait.
+  Qed.
+
+  Let is_pair_none_prop:
+    forall o,
+    IsSeq o ->
+    is_par o = None.
+  Proof.
+    intros.
+    inversion H; auto.
+  Qed.
+
+  Let is_pair_none_spec:
+    forall o,
+    is_par o = None <-> IsSeq o.
+  Proof.
+    split; auto.
+  Qed.
+
+  Definition update_nodes vs (e:event) :=
+  let (x, o) := e in
+  match is_par o with
+  | Some y => y::x::vs
+  | _ => x::vs
+  end.
+
+  (** Annotates the nodes with a phase number. *)
+
+  Definition phases := (Map_TID.t node * MN.t nat) % type.
+
+  Inductive GetPhase : tid -> nat -> phases -> Prop :=
+  | get_phase_def:
+    forall (n:node) x w ns phs,
+    Map_TID.MapsTo x n ns -> (* get the last node *)
+    MN.MapsTo n w phs -> (* get the phase number *)
+    GetPhase x w (ns, phs).
+
+  Let get_phase (x:tid) (ws:phases) :=
+  let (ns, phs) := ws in
+  match Map_TID.find x ns with
+  | Some n =>
+    match MN.find n phs with
+    | Some ph => Some ph
+    | _ => None
+    end
+  | _ => None
+  end.
+
+  Let get_phase_some:
+    forall x ws n,
+    get_phase x ws = Some n ->
+    GetPhase x n ws.
+  Proof.
+    unfold get_phase; intros.
+    destruct ws as (ns, phs).
+    destruct (Map_TID_Extra.find_rw x ns) as [(R,?)|(n',(R,?))];
+    rewrite R in *; clear R. {
+      inversion H.
+    }
+    destruct (MN_Extra.find_rw n' phs) as [(R,?)|(?,(R,?))];
+    rewrite R in *; clear R. {
+      inversion H.
+    }
+    inversion H; subst.
+    eauto using get_phase_def.
+  Qed.
+
+  Let get_phase_some_prop:
+    forall x ws n,
+    GetPhase x n ws ->
+    get_phase x ws = Some n.
+  Proof.
+    unfold get_phase; intros.
+    inversion H; subst; clear H.
+    destruct (Map_TID_Extra.find_rw x ns) as [(R,?)|(n',(R,?))];
+    rewrite R in *; clear R. {
+      contradiction H.
+      eauto using Map_TID_Extra.mapsto_to_in.
+    }
+    assert (n' = n0) by eauto using Map_TID_Facts.MapsTo_fun; subst.
+    destruct (MN_Extra.find_rw n0 phs) as [(R,?)|(?,(R,?))];
+    rewrite R in *; clear R. {
+      contradiction H2.
+      eauto using MN_Extra.mapsto_to_in.
+    }
+    assert (x0 = n) by eauto using MN_Facts.MapsTo_fun; subst.
+    trivial.
+  Qed.
+
+  Inductive SetPhase vs : phases -> tid -> nat -> phases -> Prop :=
+  | set_phase_def:
+    forall n ns ps x ph,
     MapsTo x n vs ->
-    Add vs es (x, CONTINUE) (x::vs) ((CONTINUE, (n, fresh vs))::es).
+    SetPhase vs (ns,ps) x ph (Map_TID.add x n ns, MN.add n ph ps).
+
+  Let set_phase vs (ws:phases) (x:tid) ph :=
+  let (ns,ps) := ws in
+  match lookup TID.eq_dec x vs with
+  | Some n => Some (Map_TID.add x n ns, MN.add n ph ps)
+  | _ => None
+  end.
+
+  Let set_phase_some:
+    forall vs ws x ph ws',
+    set_phase vs ws x ph = Some ws' ->
+    SetPhase vs ws x ph ws'.
+  Proof.
+    unfold set_phase; intros.
+    destruct ws as (ns,ps).
+    remember (lookup _ _ _).
+    symmetry in Heqo.
+    destruct o. {
+      apply lookup_some in Heqo.
+      inversion H; subst.
+      auto using set_phase_def.
+    }
+    inversion H.
+  Qed.
+
+  Inductive Inc vs ws x : phases -> Prop :=
+  | inc_def:
+    forall ph ws',
+    GetPhase x ph ws ->
+    SetPhase vs ws x (S ph) ws' ->
+    Inc vs ws x ws'.
+
+  Let inc vs ws x : option phases :=
+  match get_phase x ws with
+  | Some ph => set_phase vs ws x (S ph)
+  | _ => None
+  end.
+
+  Inductive Drop: phases -> tid -> phases -> Prop :=
+  | drop_def:
+    forall ns ps x,
+    Drop (ns, ps) x (Map_TID.remove x ns, ps).
+
+  Let drop (x:tid) (ws:phases) : phases := let (ns, ps) := ws in (Map_TID.remove x ns, ps).
+
+  Inductive Copy vs ws x y ws' : Prop :=
+  | copy_def:
+    forall ph,
+    GetPhase x ph ws ->
+    SetPhase vs ws y ph ws' ->
+    Copy vs ws x y ws'.
+
+  Let copy vs x y ws :=
+  match get_phase x ws with
+  | Some ph => set_phase vs ws y ph
+  | _ => None
+  end.
+
+  Inductive UpdateWP (vs:list tid) (ws:phases): event -> phases -> Prop :=
+  | update_wp_async:
+    forall x y,
+    UpdateWP vs ws (x, ASYNC y) ws
+  | update_wp_phased:
+    forall ws' x y r,
+    CanWait r ->
+    Copy vs ws x y ws' ->
+    UpdateWP vs ws (x, ASYNC_PHASED y r) ws'
+  | update_wp_signal:
+    forall x,
+    UpdateWP vs ws (x, SIGNAL) ws
+  | upate_wp_wait:
+    forall x ws',
+    Inc vs ws x ws' ->
+    UpdateWP vs ws (x, WAIT) ws'
+  | upate_wp_drop:
+    forall x ws',
+    Drop ws x ws' ->
+    UpdateWP vs ws (x, DROP) ws'
+  | upate_wp_continue:
+    forall x,
+    UpdateWP vs ws (x, CONTINUE) ws.
+
+  Definition update_wp vs (e:event) (wp:phases) : option phases :=
+  let (x, o) := e in
+  match o with
+  | ASYNC_PHASED y r =>
+    if can_wait_dec r then copy vs x y wp
+    else None
+  | WAIT => inc vs wp x
+  | DROP => Some (drop x wp)
+  | _ => Some wp
+  end.
+
+  Inductive UpdateSP (vs:list tid) (ws:phases): event -> phases -> Prop :=
+  | update_sp_async:
+    forall x y,
+    UpdateSP vs ws (x, ASYNC y) ws
+  | update_sp_phased:
+    forall ws' x y r,
+    CanSignal r ->
+    Copy vs ws x y ws' ->
+    UpdateSP vs ws (x, ASYNC_PHASED y r) ws'
+  | update_sp_signal:
+    forall x ws',
+    Inc vs ws x ws' ->
+    UpdateSP vs ws (x, SIGNAL) ws'
+  | upate_sp_wait:
+    forall x,
+    UpdateSP vs ws (x, WAIT) ws
+  | upate_sp_drop:
+    forall x ws',
+    Drop ws x ws' ->
+    UpdateSP vs ws (x, DROP) ws'
+  | upate_sp_continue:
+    forall x,
+    UpdateSP vs ws (x, CONTINUE) ws.
+
+  Definition update_sp vs (e:event) wp :=
+  let (x, o) := e in
+  match o with
+  | ASYNC_PHASED y r =>
+    if can_signal_dec r then copy vs x y wp
+    else None
+  | SIGNAL => inc vs wp x
+  | DROP => Some (drop x wp)
+  | _ => Some wp
+  end.
+
+  (* Old nodes *)
+
+  Inductive AddCEdges vs vs' : event -> list edge -> Prop :=
+  | add_c_edges_def:
+    forall x o n n',
+    MapsTo x n vs ->
+    MapsTo x n' vs' ->
+    AddCEdges vs vs' (x,o) ((n, n')::nil).
+
+  Let add_c_edges vs vs' (e:event) :=
+  let (x, o) := e in
+  match lookup TID.eq_dec x vs, lookup TID.eq_dec x vs' with
+  | Some n, Some n' => Some ((n, n'):: nil)
+  | _,_ => None
+  end.
+
+  (* Old nodes *)
+
+  Inductive AddFEdges vs vs' : event -> list (node * node) -> Prop :=
+  | add_f_edges_eq:
+    forall x nx ny y o,
+    MapsTo x nx vs ->
+    MapsTo y ny vs' ->
+    IsPar o y ->
+    AddFEdges vs vs' (x, o) ((nx, ny)::nil)
+  | fork_edge_neq:
+    forall x o,
+    IsSeq o ->
+    AddFEdges vs vs' (x, o) nil.
+
+  Let add_f_edges vs vs' (e:event) :=
+  let (x, o) := e in
+  match is_par o, lookup TID.eq_dec x vs with
+  | Some y, Some nx =>
+    match lookup TID.eq_dec y vs' with
+    | Some ny => Some ((nx, ny)::nil)
+    | _ => None
+    end
+  | _, _ => None
+  end.
+
+  Structure builder := {
+    get_nodes: list tid;
+    get_sp: phases;
+    get_wp: phases
+  }.
+
+  Definition Phase n ph (sp:phases) := MN.MapsTo n ph (snd sp).
+
+  (** Get all nodes that signaled phase [ph]. *)
+
+  Let phase ph (sp:phases) :=
+  List.omap (fun (e:node*nat) =>
+    let (n, s) := e in
+    if eq_nat_dec s ph
+    then Some n
+    else None
+  )
+  (MN.elements (snd sp)).
+
+  Inductive AddSEdges (b:builder) (vs':list tid) : event -> list (node * node) -> Prop :=
+  | add_s_edges_eq:
+    forall es x n ph,
+    GetPhase x ph (get_wp b) ->
+    MapsTo x n vs' ->
+    (forall n', List.In (n, n') es <-> Phase n' (S ph) (get_sp b)) ->
+    AddSEdges b vs' (x, WAIT) es
+  | add_s_edges_neq:
+    forall x o,
+    o <> WAIT ->
+    AddSEdges b vs' (x, o) nil.
+
+  Let add_s_edges b (vs':list tid) (e:event) :=
+  let (x, o) := e in
+  match o with
+  | WAIT =>
+    match get_phase x (get_wp b), lookup TID.eq_dec x vs' with
+    | Some ph, Some n =>
+      Some (map (fun n' => (n, n')) (phase (S ph) (get_sp b)))
+    | _, _ => None
+    end
+  | _ => Some nil
+  end.
+
+  Inductive UpdateBuilder (b:builder) : event -> builder -> Prop :=
+  | update_builder_def:
+    forall sp wp e,
+    UpdateSP (update_nodes (get_nodes b) e) (get_sp b) e sp ->
+    UpdateWP (update_nodes (get_nodes b) e) (get_wp b) e wp ->
+    UpdateBuilder b e {| get_nodes:=update_nodes (get_nodes b) e; get_sp:=sp; get_wp:=wp |}.
+
+  Let update_builder (e:event) b :=
+  let vs := update_nodes (get_nodes b) e in
+  match update_sp vs e (get_sp b), update_wp vs e (get_wp b) with
+  | Some sp, Some wp => Some {| get_nodes:=vs; get_sp:=sp; get_wp:=wp |}
+  | _, _ => None
+  end.
+
+  Structure computation_graph := {
+    c_edges : list edge;
+    f_edges : list edge;
+    s_edges : list edge
+  }.
+
+  Inductive AddEdges (b b':builder) (cg:computation_graph) (e:event) : computation_graph -> Prop :=
+  | add_edges_def:
+    forall ec ef es,
+    AddCEdges (get_nodes b) (get_nodes b') e ec ->
+    AddFEdges (get_nodes b) (get_nodes b') e ef ->
+    AddSEdges b (get_nodes b') e es -> 
+    AddEdges b b' cg e
+      {| c_edges := ec ++ c_edges cg; f_edges:= ef ++ f_edges cg; s_edges:= es ++ s_edges cg |}.
+
+  Let add_edges (b b':builder) (e:event) (cg:computation_graph) : option computation_graph :=
+  match add_c_edges (get_nodes b) (get_nodes b') e,
+        add_f_edges (get_nodes b) (get_nodes b') e,
+        add_s_edges b (get_nodes b') e with
+  | Some ec, Some ef, Some es =>
+    Some {| c_edges := ec ++ c_edges cg; f_edges:= ef ++ f_edges cg; s_edges:= es ++ s_edges cg |}
+  | _,_,_ => None
+  end.
+
+  Inductive Add : builder * computation_graph -> event -> builder * computation_graph -> Prop :=
+  | add_def:
+    forall b b' cg cg' e,
+    UpdateBuilder b e b' ->
+    AddEdges b b' cg e cg' ->
+    Add (b, cg) e (b', cg').
+
+  Definition add (e:event) (bcg:builder * computation_graph) :=
+  let (b, cg) := bcg in
+  match update_builder e b with
+  | Some b' =>
+    match add_edges b b' e cg with
+    | Some cg' => Some (b', cg')
+    | _ => None
+    end
+  | _ => None
+  end.
+
+  Definition edges cg := (c_edges cg) ++ (f_edges cg) ++ (s_edges cg).
+(*
+
 
   Ltac try_absurd := try 
       (right; unfold not; intros N;
@@ -79,13 +447,15 @@ Section Defs.
     destruct x, y; auto;
     try (destruct (TID.eq_dec t t0); auto);
     try (destruct (TID.eq_dec n n0); auto);
+    try (destruct (regmode_eq_dec r r0); subst; auto);
     try_absurd.
   Defined.
 
-  Let node_edge_eq_dec := pair_eq_dec node_eq_dec.
+  Let edge_eq_dec := pair_eq_dec node_edge_eq_dec.
 
-  Let edge_eq_dec := pair_eq_dec_2 op_eq_dec node_edge_eq_dec.
 
+
+(*
   Let phase_dec ph o :
     { Phase ph o } + { ~ Phase ph o }.
   Proof.
@@ -101,7 +471,7 @@ Section Defs.
     destruct (phase_dec ph o); auto using sync_def.
     try_absurd.
   Defined.
-
+*)
   Let wait_edge (vs:list tid) ph e :=
   if sync_dec ph e
   then Some (PREC, ((fst (snd e)), fresh vs))
@@ -276,7 +646,7 @@ Section Defs.
     }
     inversion H.
   Qed.
-
+*)
 End Defs.
 
-Extraction "ocaml/cg.ml" build to_cg.
+Extraction "ocaml/cg.ml" add.
